PhysLean/Particles/SuperSymmetry/SU5/ChargeSpectrum/Map.lean
@@ -3,8 +3,8 @@ Copyright (c) 2025 Joseph Tooby-Smith. All rights reserved.
 Released under Apache 2.0 license as described in the file LICENSE.
 Authors: Joseph Tooby-Smith
 -/
-import PhysLean.Particles.SuperSymmetry.SU5.Charges.Yukawa
-import PhysLean.Particles.SuperSymmetry.SU5.Charges.Completions
+import PhysLean.Particles.SuperSymmetry.SU5.ChargeSpectrum.Yukawa
+import PhysLean.Particles.SuperSymmetry.SU5.ChargeSpectrum.Completions
 /-!
 
 # Mapping charges from different sets
@@ -30,7 +30,7 @@ a computationaly efficient way.
 namespace SuperSymmetry
 
 namespace SU5
-namespace Charges
+namespace ChargeSpectrum
 
 variable {𝓩 𝓩1 𝓩2 : Type} [AddCommGroup 𝓩] [AddCommGroup 𝓩1] [DecidableEq 𝓩1]
   [AddCommGroup 𝓩2] [DecidableEq 𝓩2]
@@ -38,24 +38,24 @@ variable {𝓩 𝓩1 𝓩2 : Type} [AddCommGroup 𝓩] [AddCommGroup 𝓩1] [Dec
 /-- Given an additive monoid homomorphisms `f : 𝓩 →+ 𝓩1`, for a charge
   `x : Charges 𝓩`, `x.map f` is the charge of `Charges 𝓩1` obtained by mapping the elements
   of `x` by `f`. -/
-def map (f : 𝓩 →+ 𝓩1) (x : Charges 𝓩) : Charges 𝓩1 :=
+def map (f : 𝓩 →+ 𝓩1) (x : ChargeSpectrum 𝓩) : ChargeSpectrum 𝓩1 :=
   (f <$> x.1, f <$> x.2.1, x.2.2.1.image f, x.2.2.2.image f)
 
 @[simp]
-lemma map_empty (f : 𝓩 →+ 𝓩1) : map f (∅ : Charges 𝓩) = ∅ := by
+lemma map_empty (f : 𝓩 →+ 𝓩1) : map f (∅ : ChargeSpectrum 𝓩) = ∅ := by
   simp only [map, empty_qHd, Option.map_eq_map, Option.map_none, empty_qHu, empty_Q5,
     Finset.image_empty, empty_Q10]
   rfl
 
-lemma map_map (f : 𝓩 →+ 𝓩1) (g : 𝓩1 →+ 𝓩2) (x : Charges 𝓩) :
+lemma map_map (f : 𝓩 →+ 𝓩1) (g : 𝓩1 →+ 𝓩2) (x : ChargeSpectrum 𝓩) :
     map g (map f x) = map (g.comp f) x := by
   simp [map, Option.map_map, Finset.image_image]
 
 @[simp]
-lemma map_id [DecidableEq 𝓩] (x : Charges 𝓩) : map (AddMonoidHom.id 𝓩) x = x := by
+lemma map_id [DecidableEq 𝓩] (x : ChargeSpectrum 𝓩) : map (AddMonoidHom.id 𝓩) x = x := by
   simp [map, Finset.image_id]
 
-lemma map_ofFieldLabel (f : 𝓩 →+ 𝓩1) (x : Charges 𝓩) (F : FieldLabel) :
+lemma map_ofFieldLabel (f : 𝓩 →+ 𝓩1) (x : ChargeSpectrum 𝓩) (F : FieldLabel) :
     ofFieldLabel (map f x) F = (ofFieldLabel x F).image f := by
   simp [ofFieldLabel, map]
   match x with
@@ -83,7 +83,7 @@ lemma map_ofFieldLabel (f : 𝓩 →+ 𝓩1) (x : Charges 𝓩) (F : FieldLabel)
       simp
 
 lemma map_ofPotentialTerm_toFinset [DecidableEq 𝓩]
-    (f : 𝓩 →+ 𝓩1) (x : Charges 𝓩) (T : PotentialTerm) :
+    (f : 𝓩 →+ 𝓩1) (x : ChargeSpectrum 𝓩) (T : PotentialTerm) :
     (ofPotentialTerm (map f x) T).toFinset = (ofPotentialTerm x T).toFinset.image f := by
   ext i
   simp [Multiset.mem_toFinset]
@@ -174,7 +174,7 @@ lemma map_ofPotentialTerm_toFinset [DecidableEq 𝓩]
     case β => refine ⟨q2, q2_mem, rfl⟩
 
 lemma mem_map_ofPotentialTerm_iff [DecidableEq 𝓩]
-    (f : 𝓩 →+ 𝓩1) (x : Charges 𝓩) (T : PotentialTerm) :
+    (f : 𝓩 →+ 𝓩1) (x : ChargeSpectrum 𝓩) (T : PotentialTerm) :
     i ∈ (ofPotentialTerm (map f x) T) ↔ i ∈ (ofPotentialTerm x T).map f := by
   trans i ∈ (ofPotentialTerm (map f x) T).toFinset
   · simp
@@ -182,7 +182,7 @@ lemma mem_map_ofPotentialTerm_iff [DecidableEq 𝓩]
   simp
 
 lemma mem_map_ofPotentialTerm'_iff[DecidableEq 𝓩]
-    (f : 𝓩 →+ 𝓩1) (x : Charges 𝓩) (T : PotentialTerm) :
+    (f : 𝓩 →+ 𝓩1) (x : ChargeSpectrum 𝓩) (T : PotentialTerm) :
     i ∈ (ofPotentialTerm' (map f x) T) ↔ i ∈ (ofPotentialTerm' x T).map f := by
   rw [← mem_ofPotentialTerm_iff_mem_ofPotentialTerm]
   rw [mem_map_ofPotentialTerm_iff]
@@ -196,14 +196,14 @@ lemma mem_map_ofPotentialTerm'_iff[DecidableEq 𝓩]
     exact mem_ofPotentialTerm_iff_mem_ofPotentialTerm.mpr h
 
 lemma map_ofPotentialTerm'_toFinset [DecidableEq 𝓩]
-    (f : 𝓩 →+ 𝓩1) (x : Charges 𝓩) (T : PotentialTerm) :
+    (f : 𝓩 →+ 𝓩1) (x : ChargeSpectrum 𝓩) (T : PotentialTerm) :
     (ofPotentialTerm' (map f x) T).toFinset = (ofPotentialTerm' x T).toFinset.image f := by
   ext i
   simp only [Multiset.mem_toFinset, Finset.mem_image]
   rw [mem_map_ofPotentialTerm'_iff]
   simp
 
-lemma map_subset {f : 𝓩 →+ 𝓩1} {x y : Charges 𝓩} (h : x ⊆ y) :
+lemma map_subset {f : 𝓩 →+ 𝓩1} {x y : ChargeSpectrum 𝓩} (h : x ⊆ y) :
     map f x ⊆ map f y := by
   simp [map, subset_def] at *
   obtain ⟨hHd, hHu, hQ5, hQ10⟩ := h
@@ -234,7 +234,7 @@ lemma allowsTermForm_map {T} {f : 𝓩 →+ 𝓩1} {a b c : 𝓩} :
   cases T
   all_goals simp [allowsTermForm, map]
 
-lemma map_allowsTerm {f : 𝓩 →+ 𝓩1} {x : Charges 𝓩} {T : PotentialTerm}
+lemma map_allowsTerm {f : 𝓩 →+ 𝓩1} {x : ChargeSpectrum 𝓩} {T : PotentialTerm}
     (h : x.AllowsTerm T) : (map f x).AllowsTerm T := by
   rw [allowsTerm_iff_subset_allowsTermForm] at ⊢ h
   obtain ⟨a, b, c, h1⟩ := h
@@ -242,7 +242,7 @@ lemma map_allowsTerm {f : 𝓩 →+ 𝓩1} {x : Charges 𝓩} {T : PotentialTerm
   rw [← allowsTermForm_map]
   exact map_subset h1
 
-lemma map_isPhenoConstrained (f : 𝓩 →+ 𝓩1) {x : Charges 𝓩}
+lemma map_isPhenoConstrained (f : 𝓩 →+ 𝓩1) {x : ChargeSpectrum 𝓩}
     (h : x.IsPhenoConstrained) : (map f x).IsPhenoConstrained := by
   simp [IsPhenoConstrained] at ⊢ h
   rcases h with h | h | h | h | h | h | h | h
@@ -255,16 +255,16 @@ lemma map_isPhenoConstrained (f : 𝓩 →+ 𝓩1) {x : Charges 𝓩}
   · exact Or.inr (Or.inr (Or.inr (Or.inr (Or.inr (Or.inr (Or.inl (map_allowsTerm h)))))))
   · exact Or.inr (Or.inr (Or.inr (Or.inr (Or.inr (Or.inr (Or.inr ((map_allowsTerm h))))))))
 
-lemma not_isPhenoConstrained_of_map {f : 𝓩 →+ 𝓩1} {x : Charges 𝓩}
+lemma not_isPhenoConstrained_of_map {f : 𝓩 →+ 𝓩1} {x : ChargeSpectrum 𝓩}
     (h : ¬ (map f x).IsPhenoConstrained) : ¬ x.IsPhenoConstrained :=
   fun hn => h (map_isPhenoConstrained f hn)
 
 omit [DecidableEq 𝓩] in
-lemma map_isComplete_iff {f : 𝓩 →+ 𝓩1} {x : Charges 𝓩} :
+lemma map_isComplete_iff {f : 𝓩 →+ 𝓩1} {x : ChargeSpectrum 𝓩} :
     (map f x).IsComplete ↔ x.IsComplete := by
   simp [IsComplete, map]
 
-lemma map_ofYukawaTerms_toFinset {f : 𝓩 →+ 𝓩1} {x : Charges 𝓩} :
+lemma map_ofYukawaTerms_toFinset {f : 𝓩 →+ 𝓩1} {x : ChargeSpectrum 𝓩} :
     (map f x).ofYukawaTerms.toFinset = x.ofYukawaTerms.toFinset.image f := by
   simp [ofYukawaTerms]
   ext i
@@ -273,14 +273,14 @@ lemma map_ofYukawaTerms_toFinset {f : 𝓩 →+ 𝓩1} {x : Charges 𝓩} :
   rw [mem_map_ofPotentialTerm'_iff, mem_map_ofPotentialTerm'_iff]
   simp [Multiset.mem_map]
 
-lemma mem_map_ofYukawaTerms_iff {f : 𝓩 →+ 𝓩1} {x : Charges 𝓩} {i} :
+lemma mem_map_ofYukawaTerms_iff {f : 𝓩 →+ 𝓩1} {x : ChargeSpectrum 𝓩} {i} :
     i ∈ (map f x).ofYukawaTerms ↔ i ∈ x.ofYukawaTerms.map f := by
   trans i ∈ (map f x).ofYukawaTerms.toFinset
   · simp
   rw [map_ofYukawaTerms_toFinset]
   simp
 
-lemma map_ofYukawaTermsNSum_toFinset {f : 𝓩 →+ 𝓩1} {x : Charges 𝓩} {n : ℕ}:
+lemma map_ofYukawaTermsNSum_toFinset {f : 𝓩 →+ 𝓩1} {x : ChargeSpectrum 𝓩} {n : ℕ}:
     ((map f x).ofYukawaTermsNSum n).toFinset = (x.ofYukawaTermsNSum n).toFinset.image f:= by
   induction n with
   | zero => simp [ofYukawaTermsNSum]
@@ -315,19 +315,19 @@ lemma map_ofYukawaTermsNSum_toFinset {f : 𝓩 →+ 𝓩1} {x : Charges 𝓩} {n
         use b
       exact h
 
-lemma mem_map_ofYukawaTermsNSum_iff {f : 𝓩 →+ 𝓩1} {x : Charges 𝓩} {n i} :
+lemma mem_map_ofYukawaTermsNSum_iff {f : 𝓩 →+ 𝓩1} {x : ChargeSpectrum 𝓩} {n i} :
     i ∈ (map f x).ofYukawaTermsNSum n ↔ i ∈ (x.ofYukawaTermsNSum n).map f := by
   trans i ∈ ((map f x).ofYukawaTermsNSum n).toFinset
   · simp
   rw [map_ofYukawaTermsNSum_toFinset]
   simp
 
-lemma map_phenoConstrainingChargesSP_toFinset {f : 𝓩 →+ 𝓩1} {x : Charges 𝓩} :
+lemma map_phenoConstrainingChargesSP_toFinset {f : 𝓩 →+ 𝓩1} {x : ChargeSpectrum 𝓩} :
     (map f x).phenoConstrainingChargesSP.toFinset =
     x.phenoConstrainingChargesSP.toFinset.image f := by
   simp [phenoConstrainingChargesSP, map_ofPotentialTerm'_toFinset, Finset.image_union]
 
-lemma map_yukawaGeneratesDangerousAtLevel (f : 𝓩 →+ 𝓩1) {x : Charges 𝓩} (n : ℕ)
+lemma map_yukawaGeneratesDangerousAtLevel (f : 𝓩 →+ 𝓩1) {x : ChargeSpectrum 𝓩} (n : ℕ)
     (h : x.YukawaGeneratesDangerousAtLevel n) : (map f x).YukawaGeneratesDangerousAtLevel n := by
   rw [yukawaGeneratesDangerousAtLevel_iff_toFinset]
   rw [map_phenoConstrainingChargesSP_toFinset, map_ofYukawaTermsNSum_toFinset]
@@ -336,7 +336,7 @@ lemma map_yukawaGeneratesDangerousAtLevel (f : 𝓩 →+ 𝓩1) {x : Charges �
   rw [Finset.not_disjoint_iff_nonempty_inter, Finset.nonempty_iff_ne_empty]
   exact (yukawaGeneratesDangerousAtLevel_iff_toFinset _ _).mp h
 
-lemma not_yukawaGeneratesDangerousAtLevel_of_map {f : 𝓩 →+ 𝓩1} {x : Charges 𝓩}
+lemma not_yukawaGeneratesDangerousAtLevel_of_map {f : 𝓩 →+ 𝓩1} {x : ChargeSpectrum 𝓩}
     (n : ℕ) (h : ¬ (map f x).YukawaGeneratesDangerousAtLevel n) :
     ¬ x.YukawaGeneratesDangerousAtLevel n :=
   fun hn => h (map_yukawaGeneratesDangerousAtLevel f n hn)
@@ -349,7 +349,8 @@ lemma not_yukawaGeneratesDangerousAtLevel_of_map {f : 𝓩 →+ 𝓩1} {x : Char
 
 /-- The preimage of a charge `Charges 𝓩1` in `ofFinset S5 S10 ⊆ Charges 𝓩` under
   mapping charges through `f : 𝓩 →+ 𝓩1`. -/
-def preimageOfFinset (S5 S10 : Finset 𝓩) (f : 𝓩 →+ 𝓩1) (x : Charges 𝓩1) : Finset (Charges 𝓩) :=
+def preimageOfFinset (S5 S10 : Finset 𝓩) (f : 𝓩 →+ 𝓩1)
+    (x : ChargeSpectrum 𝓩1) : Finset (ChargeSpectrum 𝓩) :=
   let SHd := (S5.map ⟨Option.some, Option.some_injective 𝓩⟩ ∪ {none} : Finset (Option 𝓩)).filter
     fun y => f <$> y = x.1
   let SHu := (S5.map ⟨Option.some, Option.some_injective 𝓩⟩ ∪ {none} : Finset (Option 𝓩)).filter
@@ -360,8 +361,8 @@ def preimageOfFinset (S5 S10 : Finset 𝓩) (f : 𝓩 →+ 𝓩1) (x : Charges �
   let SQ10 : Finset (Finset 𝓩) := SQ10'.powerset.filter fun y => y.image f = x.2.2.2
   SHd.product <| SHu.product <| SQ5.product SQ10
 
-lemma preimageOfFinset_eq (S5 S10 : Finset 𝓩) (f : 𝓩 →+ 𝓩1) (x : Charges 𝓩1) :
-    preimageOfFinset S5 S10 f x = {y : Charges 𝓩 | y.map f = x ∧ y ∈ ofFinset S5 S10} := by
+lemma preimageOfFinset_eq (S5 S10 : Finset 𝓩) (f : 𝓩 →+ 𝓩1) (x : ChargeSpectrum 𝓩1) :
+    preimageOfFinset S5 S10 f x = {y : ChargeSpectrum 𝓩 | y.map f = x ∧ y ∈ ofFinset S5 S10} := by
   ext y
   match y, x with
   | (yHd, yHu, y5, y10), (xHd, xHu, x5, x10) =>
@@ -413,7 +414,7 @@ lemma preimageOfFinset_eq (S5 S10 : Finset 𝓩) (f : 𝓩 →+ 𝓩1) (x : Char
 /-- The cardiniality of the
   preimage of a charge `Charges 𝓩1` in `ofFinset S5 S10 ⊆ Charges 𝓩` under
   mapping charges through `f : 𝓩 →+ 𝓩1`. -/
-def preimageOfFinsetCard (S5 S10 : Finset 𝓩) (f : 𝓩 →+ 𝓩1) (x : Charges 𝓩1) : ℕ :=
+def preimageOfFinsetCard (S5 S10 : Finset 𝓩) (f : 𝓩 →+ 𝓩1) (x : ChargeSpectrum 𝓩1) : ℕ :=
   let SHd := (S5.map ⟨Option.some, Option.some_injective 𝓩⟩ ∪ {none} : Finset (Option 𝓩)).filter
     fun y => f <$> y = x.1
   let SHu := (S5.map ⟨Option.some, Option.some_injective 𝓩⟩ ∪ {none} : Finset (Option 𝓩)).filter
@@ -424,7 +425,7 @@ def preimageOfFinsetCard (S5 S10 : Finset 𝓩) (f : 𝓩 →+ 𝓩1) (x : Charg
   let SQ10 : Finset (Finset 𝓩) := SQ10'.powerset.filter fun y => y.image f = x.2.2.2
   SHd.card * SHu.card * SQ5.card * SQ10.card
 
-lemma preimageOfFinset_card_eq (S5 S10 : Finset 𝓩) (f : 𝓩 →+ 𝓩1) (x : Charges 𝓩1) :
+lemma preimageOfFinset_card_eq (S5 S10 : Finset 𝓩) (f : 𝓩 →+ 𝓩1) (x : ChargeSpectrum 𝓩1) :
     preimageOfFinsetCard S5 S10 f x =
     (preimageOfFinset S5 S10 f x).card := by
   rw [preimageOfFinset]
@@ -432,7 +433,7 @@ lemma preimageOfFinset_card_eq (S5 S10 : Finset 𝓩) (f : 𝓩 →+ 𝓩1) (x :
   repeat rw [Finset.card_product]
   simp [preimageOfFinsetCard, mul_assoc]
 
-end Charges
+end ChargeSpectrum
 end SU5
 
 end SuperSymmetry
