PhysLean/Particles/SuperSymmetry/SU5/ChargeSpectrum/PhenoConstrained.lean
@@ -3,7 +3,7 @@ Copyright (c) 2025 Joseph Tooby-Smith. All rights reserved.
 Released under Apache 2.0 license as described in the file LICENSE.
 Authors: Joseph Tooby-Smith
 -/
-import PhysLean.Particles.SuperSymmetry.SU5.Charges.AllowsTerm
+import PhysLean.Particles.SuperSymmetry.SU5.ChargeSpectrum.AllowsTerm
 import Mathlib.Tactic.Polyrith
 /-!
 
@@ -19,7 +19,7 @@ namespace SuperSymmetry
 
 namespace SU5
 
-namespace Charges
+namespace ChargeSpectrum
 open SuperSymmetry.SU5
 open PotentialTerm
 
@@ -27,21 +27,21 @@ variable {𝓩 : Type} [AddCommGroup 𝓩]
 
 /-- A charge is pheno-constrained if it leads to the presence of any term causing proton decay
   ` {W1, Λ, W2, K1}` or R-parity violation `{β, Λ, W2, W4, K1, K2}`. -/
-def IsPhenoConstrained (x : Charges 𝓩) : Prop :=
+def IsPhenoConstrained (x : ChargeSpectrum 𝓩) : Prop :=
   x.AllowsTerm μ ∨ x.AllowsTerm β ∨ x.AllowsTerm Λ ∨ x.AllowsTerm W2 ∨ x.AllowsTerm W4 ∨
   x.AllowsTerm K1 ∨ x.AllowsTerm K2 ∨ x.AllowsTerm W1
 
-instance decidableIsPhenoConstrained [DecidableEq 𝓩] (x : Charges 𝓩) :
+instance decidableIsPhenoConstrained [DecidableEq 𝓩] (x : ChargeSpectrum 𝓩) :
     Decidable x.IsPhenoConstrained :=
   inferInstanceAs (Decidable (x.AllowsTerm μ ∨ x.AllowsTerm β ∨ x.AllowsTerm Λ ∨ x.AllowsTerm W2
     ∨ x.AllowsTerm W4 ∨ x.AllowsTerm K1 ∨ x.AllowsTerm K2 ∨ x.AllowsTerm W1))
 
 @[simp]
 lemma not_isPhenoConstrained_empty :
-    ¬ IsPhenoConstrained (∅ : Charges 𝓩) := by
+    ¬ IsPhenoConstrained (∅ : ChargeSpectrum 𝓩) := by
   simp [IsPhenoConstrained, AllowsTerm, ofPotentialTerm_empty]
 
-lemma isPhenoConstrained_mono {x y : Charges 𝓩} (h : x ⊆ y)
+lemma isPhenoConstrained_mono {x y : ChargeSpectrum 𝓩} (h : x ⊆ y)
     (hx : x.IsPhenoConstrained) : y.IsPhenoConstrained := by
   simp [IsPhenoConstrained] at *
   rcases hx with hr | hr | hr | hr | hr | hr | hr | hr
@@ -50,16 +50,16 @@ lemma isPhenoConstrained_mono {x y : Charges 𝓩} (h : x ⊆ y)
     simp_all
 
 /-- The collection of charges of super-potential terms leading to a pheno-constrained model. -/
-def phenoConstrainingChargesSP (x : Charges 𝓩) : Multiset 𝓩 :=
+def phenoConstrainingChargesSP (x : ChargeSpectrum 𝓩) : Multiset 𝓩 :=
   x.ofPotentialTerm' μ + x.ofPotentialTerm' β + x.ofPotentialTerm' Λ +
   x.ofPotentialTerm' W2 + x.ofPotentialTerm' W4 + x.ofPotentialTerm' W1
 
 @[simp]
 lemma phenoConstrainingChargesSP_empty :
-    phenoConstrainingChargesSP (∅ : Charges 𝓩) = ∅ := by
+    phenoConstrainingChargesSP (∅ : ChargeSpectrum 𝓩) = ∅ := by
   simp [phenoConstrainingChargesSP]
 
-lemma phenoConstrainingChargesSP_mono [DecidableEq 𝓩] {x y : Charges 𝓩} (h : x ⊆ y) :
+lemma phenoConstrainingChargesSP_mono [DecidableEq 𝓩] {x y : ChargeSpectrum 𝓩} (h : x ⊆ y) :
     x.phenoConstrainingChargesSP ⊆ y.phenoConstrainingChargesSP := by
   simp only [phenoConstrainingChargesSP]
   refine Multiset.subset_iff.mpr ?_
@@ -79,18 +79,18 @@ lemma phenoConstrainingChargesSP_mono [DecidableEq 𝓩] {x y : Charges 𝓩} (h
 
 /-- The proposition which is true if the addition of a charge `q5` to a set of charegs `x` leads
   `x` to being phenomenologically constrained. -/
-def IsPhenoConstrainedQ5 [DecidableEq 𝓩] (x : Charges 𝓩) (q5 : 𝓩) : Prop :=
+def IsPhenoConstrainedQ5 [DecidableEq 𝓩] (x : ChargeSpectrum 𝓩) (q5 : 𝓩) : Prop :=
   x.AllowsTermQ5 q5 μ ∨ x.AllowsTermQ5 q5 β ∨ x.AllowsTermQ5 q5 Λ ∨ x.AllowsTermQ5 q5 W2 ∨
   x.AllowsTermQ5 q5 W4 ∨
   x.AllowsTermQ5 q5 K1 ∨ x.AllowsTermQ5 q5 K2 ∨ x.AllowsTermQ5 q5 W1
 
-lemma isPhenoConstrainedQ5_iff [DecidableEq 𝓩] (x : Charges 𝓩) (q5 : 𝓩) :
+lemma isPhenoConstrainedQ5_iff [DecidableEq 𝓩] (x : ChargeSpectrum 𝓩) (q5 : 𝓩) :
     x.IsPhenoConstrainedQ5 q5 ↔
     x.AllowsTermQ5 q5 β ∨ x.AllowsTermQ5 q5 Λ ∨ x.AllowsTermQ5 q5 W4 ∨
     x.AllowsTermQ5 q5 K1 ∨ x.AllowsTermQ5 q5 W1 := by
   simp [IsPhenoConstrainedQ5, AllowsTermQ5]
 
-instance decidableIsPhenoConstrainedQ5 [DecidableEq 𝓩] (x : Charges 𝓩) (q5 : 𝓩) :
+instance decidableIsPhenoConstrainedQ5 [DecidableEq 𝓩] (x : ChargeSpectrum 𝓩) (q5 : 𝓩) :
     Decidable (x.IsPhenoConstrainedQ5 q5) :=
   decidable_of_iff _ (isPhenoConstrainedQ5_iff x q5).symm
 
@@ -119,17 +119,17 @@ lemma isPhenoConstrained_insertQ5_iff_isPhenoConstrainedQ5 [DecidableEq 𝓩] {q
 
 /-- The proposition which is true if the addition of a charge `q10` to a set of charegs `x` leads
   `x` to being phenomenologically constrained. -/
-def IsPhenoConstrainedQ10 [DecidableEq 𝓩] (x : Charges 𝓩) (q10 : 𝓩) : Prop :=
+def IsPhenoConstrainedQ10 [DecidableEq 𝓩] (x : ChargeSpectrum 𝓩) (q10 : 𝓩) : Prop :=
   x.AllowsTermQ10 q10 μ ∨ x.AllowsTermQ10 q10 β ∨ x.AllowsTermQ10 q10 Λ ∨ x.AllowsTermQ10 q10 W2 ∨
   x.AllowsTermQ10 q10 W4 ∨
   x.AllowsTermQ10 q10 K1 ∨ x.AllowsTermQ10 q10 K2 ∨ x.AllowsTermQ10 q10 W1
 
-lemma isPhenoConstrainedQ10_iff [DecidableEq 𝓩] (x : Charges 𝓩) (q10 : 𝓩) :
+lemma isPhenoConstrainedQ10_iff [DecidableEq 𝓩] (x : ChargeSpectrum 𝓩) (q10 : 𝓩) :
     x.IsPhenoConstrainedQ10 q10 ↔ x.AllowsTermQ10 q10 Λ ∨ x.AllowsTermQ10 q10 W2 ∨
     x.AllowsTermQ10 q10 K1 ∨ x.AllowsTermQ10 q10 K2 ∨ x.AllowsTermQ10 q10 W1 := by
   simp [IsPhenoConstrainedQ10, AllowsTermQ10]
 
-instance decidableIsPhenoConstrainedQ10 [DecidableEq 𝓩] (x : Charges 𝓩) (q10 : 𝓩) :
+instance decidableIsPhenoConstrainedQ10 [DecidableEq 𝓩] (x : ChargeSpectrum 𝓩) (q10 : 𝓩) :
     Decidable (x.IsPhenoConstrainedQ10 q10) :=
   decidable_of_iff _ (isPhenoConstrainedQ10_iff x q10).symm
 
@@ -156,7 +156,7 @@ lemma isPhenoConstrained_insertQ10_iff_isPhenoConstrainedQ10 [DecidableEq 𝓩] 
     · apply isPhenoConstrained_mono _ hr
       simp [subset_def]
 
-end Charges
+end ChargeSpectrum
 
 end SU5
 
